isl/Examples.v
@@ -4,8 +4,8 @@
 From ISL Require Import Basics Norm.
 Local Open Scope string_scope.
 
-
+(*
 Lemma entl_elim_bind: forall P fk f1 (f:var) u H,
   (forall r, P r -> entails (defun f u;; ens_ H;; rs (fk r)) f1) ->
     entails (defun f u;; ens_ H;; rs (bind (ens (fun r => \[P r])) fk)) f1.
-Proof.
+Proof. *)
